$$
G(z)=\frac{z-1}{z}\mathcal Z[\frac{G_p(s)}{s}]=1-z^{-1}\mathcal Z[\frac{G_p(s)}{s}]
$$
$$
\begin{align}
a^{k}\leftrightarrow\frac{z}{z-a}&=\frac{1}{1-az^{-1}}\notag\\
    1\leftrightarrow\frac{1}{s}\leftrightarrow\frac{z}{z-1}&=\frac{1}{1-z^{-1}}\notag\\
    t\leftrightarrow\frac{1}{s^2}\leftrightarrow\frac{Tz}{(z-1)^2}&=\frac{Tz^{-1}}{(1-z^{-1})^2}\notag\\
    \frac{t^2}{2}\leftrightarrow\frac{1}{s^3} \leftrightarrow \frac{T^2z(z+1)}{2(z-1)^3}&=\frac{T^2z^{-1}(1+z^{-1})}{2(1-z^{-1})^3}\notag\\
    e^{-at}\leftrightarrow\frac{1}{s+a}\leftrightarrow\frac{z}{z-e^{aT}}&=\frac{1}{1-e^{-aT}z^{-1}}\notag   
\end{align}
$$
$$
\begin{align}
f(t-nT) &\leftrightarrow z^{-n}F(z) \quad 右移n\notag\\
f(t+nT) &\leftrightarrow z^{n}F(z) - \sum_{j=0}^{n-1}z^{n-j}f(j) \quad 左移n\notag
\end{align}
$$
$$
w变换(双线性变换)\quad
\left\{  
             \begin{array}{lr}  
            z=\frac{1+w}{1-w}   \\  
            w=\frac{z-1}{z+1}  
             \end{array}  
\right.  
$$
$$
	\begin{aligned}
		静态位置误差系数 \quad k_p&=\lim_{z\to 1}GH(z)\\ \notag
		静态速度误差系数 \quad k_v&=\frac{1}{T}\lim_{z\to 1}(z-1)GH(z)\\ \notag
		静态加速度误差系数 \quad k_p&=\frac{1}{T^2}\lim_{z\to 1}(z-1)^2GH(z)\\ \notag
	\end{aligned}
$$
![](img/4_2.png)
$$
\begin{align}
前向差分变换\quad &s=\frac{z-1}{T}\notag\\
后向差分变换\quad &s=\frac{1-z^{-1}}{T}\notag
\end{align}
$$

$$
\left\{  
\begin{array}{lr}  
	\dot{x}(t)=A_cx(t)+B_cu(t)\\
	y(t)=C_cx(t)+D_cu(t)\\   
\end{array}      
\right.  
\Longrightarrow
\left\{  
\begin{array}{lr}  
	x(k+1)=Ax(k)+Bu(k)\\
	y(t)=Cx(k)+Du(k)\\  
\end{array}      
\right. \\
$$
$$
A=e^{A_cT}\quad B=\int_0^Te^{A_cT}B_cdt\quad C=C_c\quad D=D_c
$$
![](img/10_1.png)
$$
\begin{align}
    x(k)=&\mathcal Z^{-1}[(zI-A)^{-1}z]x(0)+\mathcal Z^{-1}[(zI-A)^{-1}BU(z)]\notag\\
    y(k)=&\mathcal Z^{-1}[[C(zI-A)^{-1}B+D]U(z)]\notag
\end{align}
$$
$$
rankW_c=rank
\left[
\begin{matrix}
    B&&AB&&\cdots&&A^{n-2}B&&A^{n-1}B
\end{matrix}
\right]=n\Leftrightarrow 能控
$$
$$
rankW_0=rank
\left[
\begin{matrix}
    C&&CA&&\cdots&&CA^{n-2}&&CA^{n-1}
\end{matrix}
\right]^T=n\Leftrightarrow 能观
$$
$$rank
\left[
\begin{matrix}
    D&&CB&&\cdots&&CA^{q-1}B
\end{matrix}
\right]=m\Leftrightarrow 能观
$$
$$
\begin{align}
    状态反馈\quad &(z-z_0)(z-z_1)···(z-z_n)=|zI-A+BK|\notag\\
    输出反馈\quad &(z-z_0)(z-z_1)···(z-z_n)=|zI-A+BKC|\notag\\
    全维观测器\quad&(z-z_0)(z-z_2)···(z-z_n)=|zI-A+KC|\notag
\end{align}
$$
